Semantic verification of formula

Sample.v
@@ -72,3 +72,174 @@ Definition data1 := [ReoLogicCoq.dataPorts B 1].
 Eval compute in ReoLogicCoq.go data1 processed1 (length processed1) [].
 
 Eval compute in ReoLogicCoq.fire data1 [ReoLogicCoq.goTo nat B E].
+
+
+(* new tests - 12/04 *)
+
+Inductive statesSequencer := DA | DB | DC | DD | DE | DF | DG | D_DFIFOE | D_EFIFOF | D_FFIFOG.
+
+Instance statesEqDec : EqDec statesSequencer eq := 
+	{equiv_dec x y := 
+		match x, y with 
+		| DA,DA => in_left 
+		| DB,DB => in_left 
+    | DD,DD => in_left
+		| DC,DC => in_left 
+		| DE,DE => in_left 
+		| DF,DF => in_left 
+		| DG,DG => in_left 
+		| D_DFIFOE,D_DFIFOE => in_left 
+		| D_EFIFOF,D_EFIFOF => in_left 
+		| D_FFIFOG,D_FFIFOG => in_left 
+		| DA,DB => in_right 
+		| DA,DC => in_right 
+    | DA,DD => in_right
+		| DA,DE => in_right 
+		| DA,DF => in_right 
+		| DA,DG => in_right 
+		| DA,D_DFIFOE => in_right 
+		| DA,D_EFIFOF => in_right 
+		| DA,D_FFIFOG => in_right 
+		| DB,DA => in_right 
+		| DB,DC => in_right 
+    | DB,DD => in_right
+		| DB,DE => in_right 
+		| DB,DF => in_right 
+		| DB,DG => in_right 
+		| DB,D_DFIFOE => in_right 
+		| DB,D_EFIFOF => in_right 
+		| DB,D_FFIFOG => in_right 
+		| DC,DA => in_right 
+		| DC,DB => in_right
+    | DC,DD => in_right 
+		| DC,DE => in_right 
+		| DC,DF => in_right 
+		| DC,DG => in_right 
+		| DC,D_DFIFOE => in_right 
+		| DC,D_EFIFOF => in_right 
+		| DC,D_FFIFOG => in_right 
+		| DE,DA => in_right 
+		| DE,DB => in_right 
+    | DE,DD => in_right
+		| DE,DC => in_right 
+		| DE,DF => in_right 
+		| DE,DG => in_right 
+		| DE,D_DFIFOE => in_right 
+		| DE,D_EFIFOF => in_right 
+		| DE,D_FFIFOG => in_right 
+		| DF,DA => in_right 
+		| DF,DB => in_right 
+    | DF,DD => in_right
+		| DF,DC => in_right 
+		| DF,DE => in_right 
+		| DF,DG => in_right 
+		| DF,D_DFIFOE => in_right 
+		| DF,D_EFIFOF => in_right 
+		| DF,D_FFIFOG => in_right 
+		| DG,DA => in_right 
+		| DG,DB => in_right 
+		| DG,DC => in_right 
+    | DG,DD => in_right
+		| DG,DE => in_right 
+		| DG,DF => in_right 
+		| DG,D_DFIFOE => in_right 
+		| DG,D_EFIFOF => in_right 
+		| DG,D_FFIFOG => in_right 
+		| D_DFIFOE,DA => in_right 
+		| D_DFIFOE,DB => in_right 
+		| D_DFIFOE,DC => in_right 
+		| D_DFIFOE,DD => in_right 
+		| D_DFIFOE,DE => in_right 
+		| D_DFIFOE,DF => in_right 
+		| D_DFIFOE,DG => in_right 
+		| D_DFIFOE,D_EFIFOF => in_right 
+		| D_DFIFOE,D_FFIFOG => in_right 
+		| D_EFIFOF,DA => in_right 
+		| D_EFIFOF,DB => in_right 
+		| D_EFIFOF,DC => in_right 
+		| D_EFIFOF,DD => in_right 
+		| D_EFIFOF,DE => in_right 
+		| D_EFIFOF,DF => in_right 
+		| D_EFIFOF,DG => in_right 
+		| D_EFIFOF,D_DFIFOE => in_right 
+		| D_EFIFOF,D_FFIFOG => in_right 
+		| D_FFIFOG,DA => in_right 
+		| D_FFIFOG,DB => in_right 
+		| D_FFIFOG,DC => in_right 
+		| D_FFIFOG,DD => in_right 
+		| D_FFIFOG,DE => in_right 
+		| D_FFIFOG,DF => in_right 
+		| D_FFIFOG,DG => in_right 
+		| D_FFIFOG,D_DFIFOE => in_right 
+		| D_FFIFOG,D_EFIFOF => in_right
+    | DD,DA => in_right
+    | DD,DB => in_right 
+		| DD,DC => in_right 
+		| DD,DE => in_right 
+		| DD,DF => in_right 
+		| DD,DG => in_right 
+		| DD,D_DFIFOE => in_right 
+		| DD,D_EFIFOF => in_right 
+		| DD,D_FFIFOG => in_right  
+		end 
+	}.
+Proof.
+all:congruence.
+Defined.
+
+(* Record frame := mkframe {
+    S : set state;
+    R : set (state * state);
+    lambda : state -> name -> QArith_base.Q;
+    delta : state -> set dataConnector
+  }.
+
+  Close Scope Q_scope.
+
+  (* Model definition *)
+  Record model := mkmodel {
+    Fr  : frame;
+    V : state -> set bool*)
+(* We define the Sequencer connector *)
+Definition SequencerProgram := [ReoLogicCoq.fifo D E; ReoLogicCoq.sync E A; ReoLogicCoq.fifo E F;
+ReoLogicCoq.sync F B; ReoLogicCoq.sync F G; ReoLogicCoq.fifo G C; ReoLogicCoq.sync G A].
+
+(* experimental *)
+Definition lambdaTest (s: statesSequencer) (port: sequencerPorts) : QArith_base.Q := 1.
+
+Definition deltaSequencer (s:statesSequencer) :=
+  match s with
+  | DA => [ReoLogicCoq.dataPorts A 0;ReoLogicCoq.dataPorts A 1]
+  | DB => [ReoLogicCoq.dataPorts B 0;ReoLogicCoq.dataPorts B 1]
+  | DC => [ReoLogicCoq.dataPorts C 0;ReoLogicCoq.dataPorts C 1]
+  | DD => [ReoLogicCoq.dataPorts D 0;ReoLogicCoq.dataPorts D 1]
+  | DE => [ReoLogicCoq.dataPorts E 0;ReoLogicCoq.dataPorts E 1]
+  | DF => [ReoLogicCoq.dataPorts F 0;ReoLogicCoq.dataPorts F 1]
+  | DG => [ReoLogicCoq.dataPorts G 0;ReoLogicCoq.dataPorts G 1]
+  | D_EFIFOF => [ReoLogicCoq.fifoData E 0 F;ReoLogicCoq.fifoData E 1 F]
+  | D_FFIFOG => [ReoLogicCoq.fifoData F 0 G;ReoLogicCoq.fifoData F 1 G]
+  | D_DFIFOE => [ReoLogicCoq.fifoData D 0 E;ReoLogicCoq.fifoData D 1 E]
+  end.
+
+Definition frame1 := ReoLogicCoq.mkframe [DA;DB;DC;DD;DE;DF;DG;D_DFIFOE;D_EFIFOF;D_FFIFOG] 
+                    [(DD,D_DFIFOE);(D_DFIFOE,DE);(DE,DA);(DE,D_EFIFOF);(D_EFIFOF,DF);(DF,DB);(DF,D_FFIFOG);
+                      (D_FFIFOG,DG);(DG,DD)] lambdaTest deltaSequencer.
+
+Definition valuationTest (s: statesSequencer) (p : Prop) := false.
+
+Definition model1 := ReoLogicCoq.mkmodel frame1 valuationTest.
+
+Definition pi := ReoLogicCoq.sProgram SequencerProgram.
+
+Definition t := [ReoLogicCoq.dataPorts D 1].
+
+
+Eval compute in ReoLogicCoq.singleFormulaVerify model1 
+( ReoLogicCoq.box t pi (ReoLogicCoq.diamond t pi 
+    (ReoLogicCoq.proposition sequencerPorts nat True))) t.
+
+Eval compute in ReoLogicCoq.singleFormulaVerify model1 
+( ReoLogicCoq.box t pi (ReoLogicCoq.proposition sequencerPorts nat True)) t.
+
+Eval compute in ReoLogicCoq.RTC model1.
+
